---
title: "1.2 Problems and conditioning"
editor:
    render-on-save: true
---

## Example 1.2.4

Find the roots of the quadratic polynomial

$$
at^2 + bt + c = 0.
$$

Setting the first root to $r_1$ and differentiating with respect to $a$ while
holding $b$ and $c$ constant gives

$$
r^2_1 + 2ar_1\left(\frac{dr_1}{da}\right) + b \frac{dr_1}{da} = 0.
$$

Solve for the derivative.

$$
\frac{dr_1}{da} = \frac{-r_1^2}{2ar_1 + b}
$$ {#eq-1.2.12}

$r_1$ is computed by the quadratic equation:

$$
r_1 = \frac{-b + \sqrt{b^2 - 4ac}}{2a}.
$$ {#eq-r_1-quad}

Rearranging yields

$$
2ar_1 + b = \sqrt{b^2 - 4ac}
$$ {#eq-r_1-quad-mod}

Using the quadratic equation, the solution for $r_2$ is

$$
r_2 = \frac{-b - \sqrt{b^2 - 4ac}}{2a}.
$$ {#eq-r_2-quad}

Subtracting @eq-r_2-quad from @eq-r_1-quad yields

$$
\begin{align}
r_1 - r_2 = & \frac{-b + \sqrt{b^2 - 4ac}}{2a} - \frac{-b - \sqrt{b^2 - 4ac}}{2a} \\
= & \frac{\sqrt{b^2 - 4ac}}{a}.
\end{align}
$$

Rearranging,

$$
a\left(r_1 - r_2\right) = \sqrt{b^2 - 4ac}
$$ {#eq-simple-r1_-r_2}

Taking the absolute values of @eq-r_1-quad-mod and @eq-simple-r1_-r_2, and
equating yields

$$
\lvert 2ar_1 + b \rvert = \lvert \sqrt{b^2 - 4ac} \rvert= \lvert a\left(r_1 - r_2\right) \rvert.
$$

Absolute values are required because none of the expressions are guaranteed to
be positive. Taking magnitudes ensures the equality holds in all cases.
